Proved more of Clight_safety.
start_thread and resume_thread cases are left.

concurrency/common/ClightSemantincsForMachines.v
@@ -31,6 +31,7 @@ Require Import VST.veric.Clightnew_coop.
 Require Import VST.veric.Clight_core.
 Require Import VST.veric.Clightcore_coop. 
 Require Import VST.sepcomp.event_semantics.
+Require Import VST.veric.Clight_sim.
 
 Section ClightSEM.
   Definition F: Type := fundef.
@@ -99,5 +100,103 @@ Section ClightSEM.
 
   Instance ClightSem ge : Semantics :=
     { semG := G; semC := state; semSem := CLC_evsem ge; the_ge := ge }.
-  
+
+  (* extending Clight_sim to event semantics *)
+Inductive ev_star ge: state -> mem -> _ -> state -> mem -> Prop :=
+  | ev_star_refl: forall s m,
+      ev_star ge s m nil s m
+  | ev_star_step: forall s1 m1 ev1 s2 m2 ev2 s3 m3,
+      ev_step (CLC_evsem ge) s1 m1 ev1 s2 m2 -> ev_star ge s2 m2 ev2 s3 m3 ->
+      ev_star ge s1 m1 (ev1 ++ ev2) s3 m3.
+
+Lemma ev_star_one:
+  forall ge s1 m1 ev s2 m2, ev_step (CLC_evsem ge) s1 m1 ev s2 m2 -> ev_star ge s1 m1 ev s2 m2.
+Proof.
+  intros. rewrite <- (app_nil_r ev). eapply ev_star_step; eauto. apply ev_star_refl.
+Qed.
+
+Lemma ev_star_two:
+  forall ge s1 m1 ev1 s2 m2 ev2 s3 m3,
+  ev_step (CLC_evsem ge) s1 m1 ev1 s2 m2 -> ev_step (CLC_evsem ge) s2 m2 ev2 s3 m3 ->
+  ev_star ge s1 m1 (ev1 ++ ev2) s3 m3.
+Proof.
+  intros. eapply ev_star_step; eauto. apply ev_star_one; auto.
+Qed.
+
+Lemma ev_star_trans:
+  forall ge {s1 m1 ev1 s2 m2}, ev_star ge s1 m1 ev1 s2 m2 ->
+  forall {ev2 s3 m3}, ev_star ge s2 m2 ev2 s3 m3 -> ev_star ge s1 m1 (ev1 ++ ev2) s3 m3.
+Proof.
+  induction 1; intros; auto.
+  rewrite <- app_assoc.
+  eapply ev_star_step; eauto.
+Qed.
+
+
+Inductive ev_plus ge: state -> mem -> _ -> state -> mem -> Prop :=
+  | ev_plus_left: forall s1 m1 ev1 s2 m2 ev2 s3 m3,
+      ev_step (CLC_evsem ge) s1 m1 ev1 s2 m2 -> ev_star ge s2 m2 ev2 s3 m3 ->
+      ev_plus ge s1 m1 (ev1 ++ ev2) s3 m3.
+
+Lemma ev_plus_one:
+  forall ge s1 m1 ev s2 m2, ev_step (CLC_evsem ge) s1 m1 ev s2 m2 -> ev_plus ge s1 m1 ev s2 m2.
+Proof.
+  intros. rewrite <- (app_nil_r ev). eapply ev_plus_left; eauto. apply ev_star_refl.
+Qed.
+
+Lemma ev_plus_two:
+  forall ge s1 m1 ev1 s2 m2 ev2 s3 m3,
+  ev_step (CLC_evsem ge) s1 m1 ev1 s2 m2 -> ev_step (CLC_evsem ge) s2 m2 ev2 s3 m3 ->
+  ev_plus ge s1 m1 (ev1 ++ ev2) s3 m3.
+Proof.
+  intros. eapply ev_plus_left; eauto. apply ev_star_one; auto.
+Qed.
+
+Lemma ev_plus_star: forall ge s1 m1 ev s2 m2, ev_plus ge s1 m1 ev s2 m2 -> ev_star ge s1 m1 ev s2 m2.
+Proof.
+  intros. inv H. eapply ev_star_step; eauto.
+Qed.
+
+Lemma ev_plus_trans:
+  forall ge {s1 m1 ev1 s2 m2}, ev_plus ge s1 m1 ev1 s2 m2 ->
+  forall {ev2 s3 m3}, ev_plus ge s2 m2 ev2 s3 m3 -> ev_plus ge s1 m1 (ev1 ++ ev2) s3 m3.
+Proof.
+  intros.
+  inv H.
+  rewrite <- app_assoc.
+  eapply ev_plus_left. eauto.
+  eapply ev_star_trans; eauto.
+  apply ev_plus_star. auto.
+Qed.
+
+Lemma ev_star_plus_trans:
+  forall ge {s1 m1 ev1 s2 m2}, ev_star ge s1 m1 ev1 s2 m2 ->
+  forall {ev2 s3 m3}, ev_plus ge s2 m2 ev2 s3 m3 -> ev_plus ge s1 m1 (ev1 ++ ev2) s3 m3.
+Proof.
+  intros. inv H. auto.
+  rewrite <- app_assoc.
+  eapply ev_plus_left; eauto.
+  eapply ev_star_trans; eauto. apply ev_plus_star; auto.
+Qed.
+
+Lemma ev_plus_star_trans:
+  forall ge {s1 m1 ev1 s2 m2}, ev_plus ge s1 m1 ev1 s2 m2 ->
+  forall {ev2 s3 m3}, ev_star ge s2 m2 ev2 s3 m3 -> ev_plus ge s1 m1 (ev1 ++ ev2) s3 m3.
+Proof.
+  intros.
+  inv H.
+  rewrite <- app_assoc.
+  eapply ev_plus_left; eauto. eapply ev_star_trans; eauto.
+Qed.
+
+  Lemma Clight_new_ev_sim : forall ge c1 m ev c1' m',
+    event_semantics.ev_step (@semSem (Clight_newSem ge)) c1 m ev c1' m' ->
+    forall c2, match_states c1 (fst (CC'.CC_state_to_CC_core c2)) ->
+    exists c2', ev_plus ge c2 m ev c2' m' /\
+      match_states c1' (fst (CC'.CC_state_to_CC_core c2')).
+  Proof.
+    (* based on Clight_sim.Clightnew_Clight_sim_eq_noOrder_SSplusConclusion *)
+  Admitted.
+
+
 End ClightSEM.
